CausalModels/DAG_Adjacency.v
@@ -1,0 +1,93 @@
+From Utils Require Import Lists.
+From Utils Require Import Logic.
+
+From Coq Require Export Init.Nat.
+From Coq Require Export Lists.List.
+From Coq Require Export Bool.Bool.
+From Coq Require Export Arith.PeanoNat.
+Require Import Coq.Program.Wf.
+
+Import ListNotations.
+
+From CausalModels Require Import DAG_Basics.
+
+
+(* this file defines an adjacency list representation of DAGs and proves its relationship
+   to the vertices and edges representation. *)
+
+(* [(node 1, all nodes to which node 1 has edges), (node 2, ...), ...] *)
+Definition adj_list : Type := list (node * nodes).
+
+(* neighbors of a node s are all nodes to which s has directed edges (immediate children of s) *)
+Fixpoint neighbors_of_node (s: node) (E: edges) : nodes :=
+  match E with
+  | [] => []
+  | h :: t => match h with
+              | (u, v) => if (u =? s) then v :: neighbors_of_node s t else neighbors_of_node s t
+              end
+  end.
+
+Lemma neighbors_vs_edges: forall u v: node, forall E: edges,
+  member v (neighbors_of_node u E) = true <-> member_edge (u, v) E = true.
+Proof.
+  intros u v E.
+  split.
+  - intros H. induction E as [| h t IH].
+    + simpl. simpl in H. apply H.
+    + simpl. destruct (eqbedge h (u, v)) as [|] eqn:Hedge.
+      * reflexivity.
+      * apply IH. simpl in H. destruct h as [a b].
+        simpl in Hedge. destruct (a =? u) as [|] eqn:Hau.
+        -- simpl in Hedge. simpl in H. rewrite Hedge in H. apply H.
+        -- apply H.
+  - intros H. induction E as [| h t IH].
+    + simpl. simpl in H. apply H.
+    + simpl. destruct h as [a b]. simpl in H.
+      destruct (a =? u) as [|] eqn:Hau.
+      * simpl in H. simpl. destruct (b =? v) as [|] eqn:Hbv.
+        -- reflexivity.
+        -- apply IH. apply H.
+      * simpl in H. apply IH. apply H.
+Qed.
+
+Example neighbors_of_3: neighbors_of_node 3 E = [2; 1].
+Proof. reflexivity. Qed.
+
+(* compute the neighbors of each node and append together into an adjacency list *)
+Fixpoint get_adjacency_list (V: nodes) (E: edges) : adj_list :=
+  match V with
+  | [] => []
+  | h :: t => [(h, neighbors_of_node h E)] ++ get_adjacency_list t E
+  end.
+
+Compute get_adjacency_list V E.
+
+Theorem adjacency_list_equiv: forall V neighbors: nodes, forall E: edges, forall u v: node, 
+  (neighbors = neighbors_of_node u E) ->
+  ((In (u, neighbors) (get_adjacency_list V E) /\ In v neighbors) <-> (In (u, v) E /\ In u V)).
+Proof.
+  intros V neighbors E u v.
+  intros Hneighbors.
+  split.
+  - intros [Hadj Hv]. split.
+    -- induction V as [| h t IH].
+        + simpl in Hadj. exfalso. apply Hadj.
+        + simpl in Hadj. destruct Hadj as [Hadj | Hadj].
+          * injection Hadj as Hhu Hnb. 
+            rewrite <- Hnb in Hv. apply member_In_equiv in Hv. apply neighbors_vs_edges in Hv.
+            apply member_edge_In_equiv in Hv. rewrite Hhu in Hv. apply Hv.
+          * apply IH. apply Hadj.
+    -- induction V as [| h t IH].
+        + simpl. simpl in Hadj. apply Hadj.
+        + simpl. simpl in Hadj. destruct Hadj as [Hadj | Hadj].
+          * injection Hadj as Hhu Hnb. left. apply Hhu.
+          * right. apply IH. apply Hadj. 
+  - intros H. split.
+    + induction V as [| h t IH].
+      * simpl. simpl in H. destruct H as [_ H]. apply H.
+      * simpl in H. destruct H as [H1 [H2 | H3]].
+        -- rewrite -> H2. simpl. left. rewrite Hneighbors. reflexivity.
+        -- simpl. right. apply IH. split. apply H1. apply H3.
+    + destruct H as [H _]. apply member_edge_In_equiv in H. apply neighbors_vs_edges in H.
+      apply member_In_equiv in H. rewrite <- Hneighbors in H. apply H.
+Qed.
