CausalModels/DAG_TopologicalSort.v
@@ -1,0 +1,514 @@
+From CausalModels Require Import DAG_Basics.
+From CausalModels Require Import DAG_CycleDetection.
+From CausalModels Require Import DAG_Descendants.
+From Utils Require Import Lists.
+From Utils Require Import Logic.
+From Coq Require Import Arith.EqNat. Import Nat.
+From Coq Require Import Lia.
+
+Import ListNotations.
+
+
+Definition get_indegree (u: node) (G: graph): nat :=
+  length (find_parents u G).
+
+Definition get_indegree_zero (G: graph): nodes :=
+  match G with
+  | (V, E) => filter (fun v => (get_indegree v G) =? 0) V
+  end.
+
+Fixpoint construct_path (G: graph) (p: path) (iters: nat) : path :=
+  match iters with
+  | 0 => p
+  | S iters' => match p with
+                | (u, v, l) => match (find_parents u G) with
+                               | [] => p
+                               | h :: t => (construct_path G (h, v, u :: l) iters')
+                               end
+                end
+  end.
+
+Definition contains_any_node (G: graph): bool :=
+  match G with
+  | (V, E) => negb (eqblist V [])
+  end.
+
+Theorem constructed_path_in_graph: forall (G: graph) (p: path) (iters: nat),
+  G_well_formed G = true -> is_directed_path_in_graph p G = true -> is_directed_path_in_graph (construct_path G p iters) G = true.
+Proof.
+  intros G p iters Hwf H.
+  generalize dependent p. induction iters as [| iters' IH].
+  - intros p H. simpl. apply H.
+  - intros p H. destruct p as [[u v] l]. simpl. destruct (find_parents u G) as [| h t] eqn:HP.
+    + apply H.
+    + specialize IH with (p := (h, v, u :: l)). apply IH.
+      simpl. apply split_and_true. split.
+      * assert (Hedge: edge_in_graph (h, u) G = true).
+        { apply edge_from_parent_to_child. rewrite HP. simpl. left. reflexivity. }
+        apply edge_in_graph_then_is_edge in Hedge. apply Hedge. apply Hwf.
+      * apply H.
+Qed.
+
+Theorem constructed_path_adds_length_iters: forall (G: graph) (p: path) (iters: nat),
+  G_well_formed G = true /\ is_path_in_graph p G = true /\ get_indegree_zero G = []
+  -> measure_path (construct_path G p iters) = (measure_path p) + iters.
+Proof.
+  intros G p iters [Hwf [Hpath Hindeg]].
+  generalize dependent p. induction iters as [| iters' IH].
+  - intros p Hpath. simpl. rewrite add_0_r. reflexivity.
+  - intros p Hpath. destruct p as [[u v] l]. simpl. destruct (find_parents u G) as [| h t] eqn:HP.
+    + (* contradiction: u should be in get_indegree_zero G = [] *)
+      assert (contra: In u (get_indegree_zero G)).
+      { destruct G as [V E]. unfold get_indegree_zero.
+        apply filter_true. split.
+        - assert (Hu: node_in_graph u (V, E) = true).
+          { apply first_node_in_path_in_graph with (e := v) (l := l). unfold is_path_in_graph in Hpath. apply Hpath. }
+          simpl in Hu. apply member_In_equiv. apply Hu.
+        - unfold get_indegree. rewrite HP. simpl. reflexivity. }
+      rewrite Hindeg in contra. exfalso. simpl in contra. apply contra.
+    + specialize IH with (p := (h, v, u :: l)). rewrite IH.
+      * simpl. lia.
+      * destruct G as [V E]. simpl. unfold is_path_in_graph in Hpath. simpl in Hpath.
+        rewrite Hpath.
+        assert (Hhu: edge_in_graph (h, u) (V, E) = true).
+        { apply edge_from_parent_to_child. rewrite HP. simpl. left. reflexivity. }
+        simpl in Hhu. rewrite Hhu.
+        assert (Hnode: node_in_graph h (V, E) = true /\ node_in_graph u (V, E) = true).
+        { apply edge_corresponds_to_nodes_in_well_formed. split.
+          - apply Hwf.
+          - simpl. apply Hhu. }
+        simpl in Hnode. destruct Hnode as [Hh Hu]. rewrite Hh. rewrite Hu. simpl. reflexivity.
+Qed.
+
+Theorem pigeonhole: forall (V: nodes) (V': nodes),
+  (forall (u: node), In u V' -> In u V) /\ (length V < length V') -> exists (v: node), (count v V' > 1).
+Proof.
+  intros V V'. intros [Hu Hlen].
+  generalize dependent V. induction V' as [| h' t' IH].
+  - intros V Hu Hlen. simpl in Hlen. lia.
+  - intros V Hu Hlen. destruct (member h' t') as [|] eqn:Hmem.
+    + exists h'. simpl. rewrite eqb_refl.
+      assert (Hc: count h' t' >= 1).
+      { apply member_count_at_least_1. apply member_In_equiv. apply Hmem. }
+      lia.
+    + specialize IH with (V := (filter (fun v : nat => negb (v =? h')) V)).
+      assert (H: exists v : node, count v t' > 1).
+      { apply IH.
+        - intros u Hmem2. apply filter_true. split.
+          + apply Hu with (u := u). simpl. right. apply Hmem2.
+          + destruct (u =? h') as [|] eqn:H.
+            * apply eqb_eq in H. rewrite H in Hmem2. apply member_In_equiv in Hmem2. rewrite Hmem2 in Hmem. discriminate Hmem.
+            * simpl. reflexivity.
+        - assert (Hlen': S (length (filter (fun v : nat => negb (v =? h')) V)) <= length V).
+          { apply filter_length_membership. apply Hu with (u := h'). simpl. left. reflexivity. }
+          simpl in Hlen. apply succ_lt_mono. apply le_lt_trans with (m := (length V)).
+          + apply Hlen'.
+          + apply Hlen. }
+      destruct H as [v H]. exists v. simpl. destruct (h' =? v) as [|] eqn:Hhv.
+      -- lia.
+      -- apply H.
+Qed.
+
+Theorem acyclic_has_indegree_zero: forall (G: graph),
+  G_well_formed G = true /\ contains_any_node G = true /\ contains_cycle G = false
+  -> exists u, ((node_in_graph u G) && (get_indegree u G =? 0)) = true.
+Proof.
+  intros G [HGwf [Hnode Hcyc]].
+  destruct G as [V E] eqn: HG.
+  destruct (get_indegree_zero (V, E)) as [| h t] eqn:Hindeg.
+  - (* assume there are 0 nodes with indegree 0. Show a contradiction by showing that G is cyclic. *)
+    destruct V as [| v V'] eqn:HV.
+    + simpl in Hnode. discriminate Hnode.
+    + destruct (get_indegree v G) as [| n'] eqn:Hvindeg.
+      * exists v. simpl. rewrite eqb_refl. rewrite <- HG. rewrite Hvindeg. rewrite eqb_refl. reflexivity.
+      * unfold get_indegree in Hvindeg. apply length_member in Hvindeg. destruct Hvindeg as [p Hp].
+        apply edge_from_parent_to_child in Hp.
+        assert (HpV: node_in_graph p G = true /\ node_in_graph v G = true).
+        { apply edge_corresponds_to_nodes_in_well_formed. split. rewrite HG. apply HGwf. apply Hp. }
+        destruct HpV as [HpV _].
+        remember (construct_path G (p, v, []) (length V)) as cycle. (* extend (p, v) backwards |V| times *)
+        assert (Hpath: is_directed_path_in_graph cycle G = true).
+        { rewrite Heqcycle. apply constructed_path_in_graph. rewrite HG. apply HGwf. rewrite HG. simpl.
+          rewrite HG in HpV. simpl in HpV. rewrite HpV. rewrite eqb_refl.
+          rewrite HG in Hp. simpl in Hp. rewrite Hp. simpl. reflexivity. }
+        assert (Hrepeat: exists (r: node), (count r ([path_start cycle; path_end cycle] ++ (path_int cycle)) > 1)).
+        { apply pigeonhole with (V := V). split.
+          - intros x Hx.
+            assert (Heq: node_in_graph x G = true).
+            { apply nodes_in_graph_in_V with (p := cycle). split.
+              - unfold node_in_path. simpl in Hx.
+                destruct Hx as [Hs | [He | Hint]].
+                + rewrite Hs. rewrite eqb_refl. simpl. reflexivity.
+                + rewrite He. rewrite eqb_refl. simpl.
+                  apply split_orb_true. left. apply split_orb_true. right. reflexivity.
+                + apply member_In_equiv in Hint. rewrite Hint. apply split_orb_true. right. reflexivity.
+              - apply directed_path_is_path. apply Hpath. }
+            rewrite HG in Heq. rewrite <- HV in Heq. simpl in Heq. apply member_In_equiv. apply Heq.
+          - assert (Hlen: measure_path cycle = 2 + (length V)).
+            { rewrite Heqcycle. apply constructed_path_adds_length_iters. repeat split.
+              - rewrite HG. apply HGwf.
+              - rewrite HG. simpl. rewrite eqb_refl.
+                assert (Hmemp: node_in_graph p G = true /\ node_in_graph v G = true).
+                { apply edge_corresponds_to_nodes_in_well_formed. split.
+                  - rewrite HG. apply HGwf.
+                  - apply Hp. } destruct Hmemp as [Hmemp _].
+                rewrite HG in Hmemp. simpl in Hmemp. rewrite Hmemp. rewrite HG in Hp. simpl in Hp. rewrite Hp.
+                simpl. reflexivity.
+              - rewrite HG. apply Hindeg. }
+            destruct cycle as [[s e] l]. unfold measure_path in Hlen. simpl.
+            apply add_cancel_l in Hlen. rewrite Hlen. lia. }
+        assert (Hcycle: ~(acyclic_path_2 cycle)).
+        { unfold not. intros H. apply acyclic_path_correct in H. destruct Hrepeat as [r Hrepeat].
+          apply acyclic_path_intermediate_nodes with (x := r) in H. destruct H as [H0 | H1].
+          - rewrite H0 in Hrepeat. lia.
+          - rewrite H1 in Hrepeat. lia. }
+        assert (contra: contains_cycle G = true).
+        { apply contains_cycle_true_correct. exists cycle. split.
+          - apply Hpath.
+          - apply Hcycle. }
+        rewrite HG in contra. rewrite Hcyc in contra. discriminate contra.
+  - exists h.
+    unfold get_indegree_zero in Hindeg.
+    assert (Hh: In h (filter
+           (fun v : node =>
+            get_indegree v (V, E) =? 0) V)). { rewrite Hindeg. simpl. left. reflexivity. }
+    apply filter_true in Hh. unfold node_in_graph. rewrite <- member_In_equiv in Hh.
+    destruct Hh as [HhV Hhdeg]. rewrite HhV. rewrite Hhdeg. reflexivity.
+Qed.
+
+Fixpoint topological_sort_helper (G: graph) (iters: nat) : option nodes :=
+  match iters with
+  | 0 => Some []
+  | S iters' => let ind := get_indegree_zero G in
+                match ind with
+                | [] => None (* G contains cycle *)
+                | h :: t => let rec := topological_sort_helper (remove_node_from_graph G h) iters' in
+                            match rec with
+                            | None => None
+                            | Some r => Some (h :: r)
+                            end
+                end
+  end.
+
+Definition topological_sort (G: graph) : option nodes :=
+  match G with
+  | (V, E) => topological_sort_helper G (length V)
+  end.
+
+Definition V_topo: nodes := [3; 1; 2; 0; 4; 5].
+Definition E_topo: edges := [(5, 0); (5, 2); (2, 3); (3, 1); (4, 0); (4, 1)].
+
+Example toposort_1: topological_sort (V_topo, E_topo) = Some [4; 5; 2; 3; 1; 0].
+Proof. reflexivity. Qed.
+
+Lemma topo_sort_subgraph: forall (G: graph) (u: node) (ts: nodes),
+  G_well_formed G = true /\ node_in_graph u G = true
+  -> topological_sort G = Some (u :: ts) -> topological_sort (remove_node_from_graph G u) = Some ts.
+Proof.
+  intros [V E] u ts [Hwf Hu] H.
+  unfold topological_sort in H.
+  destruct (length V) as [| l'] eqn:Hlen.
+  - simpl in H. inversion H.
+  - simpl in H. destruct (get_indegree_zero (V, E)) as [| h t] eqn:Hind.
+    + unfold get_indegree_zero in Hind. rewrite Hind in H. discriminate H.
+    + unfold get_indegree_zero in Hind. rewrite Hind in H. 
+      destruct (topological_sort_helper (remove_node h V, remove_associated_edges h E) l') as [r|] eqn:Hr.
+      * inversion H. unfold topological_sort. simpl. rewrite <- H1.
+        assert (Hlen': length V = S (length (remove_node h V))).
+        { apply remove_node_from_well_formed with (E := E). split.
+          - rewrite H1. apply Hu.
+          - apply Hwf. }
+        rewrite Hlen in Hlen'. inversion Hlen'. rewrite <- H3. rewrite <- H2. apply Hr.
+      * discriminate H.
+Qed.
+
+Lemma topo_sort_exists_for_acyclic_helper: forall (G: graph) (iters: nat),
+  G_well_formed G = true /\ contains_any_node G = true /\ iters <= num_nodes G ->
+  contains_cycle G = false
+  -> exists sorted: nodes, topological_sort_helper G iters = Some sorted.
+Proof.
+  intros G iters. intros [Hwf [Hnode Hiters]].
+  intros Hcyc.
+  generalize dependent G. induction iters as [| iters' IH].
+  + intros G Hwf Hnode Hiters Hcyc. simpl. exists []. reflexivity.
+  + intros [V E] Hwf Hnode Hiters Hcyc. simpl. destruct (filter (fun v : node => get_indegree v (V, E) =? 0) V) as [| h t] eqn:Hind.
+    * assert (contra: exists u, ((node_in_graph u (V, E)) && (get_indegree u (V, E) =? 0)) = true).
+      { apply acyclic_has_indegree_zero. repeat split.
+        - apply Hwf.
+        - apply Hnode.
+        - apply Hcyc. }
+      destruct contra as [u contra].
+      assert (contra': In u (filter (fun v : node => get_indegree v (V, E) =? 0) V)).
+      { apply filter_true. apply split_and_true in contra. simpl in contra. rewrite <- member_In_equiv. apply contra. }
+      rewrite Hind in contra'. exfalso. simpl in contra'. apply contra'.
+    * destruct iters' as [| iters''] eqn:Hiters'.
+      -- simpl. exists [h]. reflexivity.
+      -- specialize IH with (G := (remove_node h V, remove_associated_edges h E)).
+         assert (Hlen: length V = S (length (remove_node h V))).
+          { apply remove_node_from_well_formed with (E := E). split.
+            - simpl. assert (H: In h (filter (fun v : node => get_indegree v (V, E) =? 0) V)).
+              { rewrite Hind. simpl. left. reflexivity. }
+              apply filter_true in H. destruct H as [H _]. apply member_In_equiv. apply H.
+            - apply Hwf. }
+      assert (H: exists sorted : nodes,
+          topological_sort_helper (remove_node_from_graph (V, E) h) iters' = Some sorted).
+      { rewrite Hiters'. apply IH.
+        - apply remove_node_preserves_well_formed with (u := h) in Hwf. simpl in Hwf. apply Hwf.
+        - simpl. simpl in Hiters.
+          rewrite Hlen in Hiters. destruct (remove_node h V) as [| h' t'].
+          + simpl in Hiters. lia.
+          + simpl. reflexivity.
+        - simpl. simpl in Hiters. lia.
+        - apply remove_node_preserves_acyclic with (u := h) in Hcyc. apply Hcyc. }
+      destruct H as [r H]. simpl in H. rewrite Hiters' in H. rewrite H. exists (h :: r). reflexivity.
+Qed.
+
+Lemma topo_sort_exists_for_acyclic: forall (G: graph),
+  G_well_formed G = true /\ contains_cycle G = false -> exists sorted: nodes, topological_sort G = Some sorted.
+Proof.
+  intros [V E].
+  intros [Hwf Hcyc].
+  unfold topological_sort. destruct (length V) as [| l'] eqn:Hlen.
+  + simpl. exists []. reflexivity.
+  + apply topo_sort_exists_for_acyclic_helper.
+    * repeat split.
+      -- apply Hwf.
+      -- simpl. destruct V as [| h t].
+         ++ simpl in Hlen. discriminate Hlen.
+         ++ simpl. reflexivity.
+      -- simpl. rewrite Hlen. lia.
+    * apply Hcyc.
+Qed.
+
+Lemma topo_sort_length_correct_helper: forall (G: graph) (iters: nat) (sorted: nodes),
+  topological_sort_helper G iters = Some sorted -> length sorted = iters.
+Proof.
+  intros G iters sorted H.
+  generalize dependent G. generalize dependent sorted. induction iters as [| iters' IH].
+  - intros sorted G H. simpl in H. inversion H. simpl. reflexivity.
+  - intros sorted G H. simpl in H. destruct (get_indegree_zero G) as [| h t].
+    + discriminate H.
+    + destruct (topological_sort_helper (remove_node_from_graph G h) iters') as [r|] eqn:Hr.
+      * specialize IH with (sorted := r) (G := (remove_node_from_graph G h)).
+        apply IH in Hr. inversion H. simpl. rewrite Hr. reflexivity.
+      * discriminate H.
+Qed.
+
+Lemma topo_sort_length_correct: forall (G: graph) (sorted: nodes),
+  topological_sort G = Some sorted -> length sorted = num_nodes G.
+Proof.
+  intros G sorted H.
+  unfold topological_sort in H. destruct G as [V E].
+  apply topo_sort_length_correct_helper in H. simpl. apply H.
+Qed.
+
+Lemma topo_sort_contains_nodes_helper: forall (G: graph) (iters: nat) (sorted: nodes),
+  iters >= num_nodes G /\ topological_sort_helper G iters = Some sorted ->
+  forall (u: node), (In u sorted <-> node_in_graph u G = true).
+Proof.
+  intros G iters sorted [Hiters Hts].
+  intros u. split.
+  - intros Hmem. generalize dependent G. generalize dependent sorted.
+    induction iters as [| iters' IH].
+    + intros sorted Hmem G Hiters Hts. simpl in Hts. inversion Hts. rewrite <- H0 in Hmem. simpl in Hmem.
+      exfalso. apply Hmem.
+    + intros sorted Hmem G Hiters Hts. simpl in Hts. destruct (get_indegree_zero G) as [| h t] eqn:Hd.
+      * discriminate Hts.
+      * destruct (topological_sort_helper (remove_node_from_graph G h) iters') as [r|] eqn:Hr.
+        -- inversion Hts. rewrite <- H0 in Hmem. simpl in Hmem.
+           assert (Hmemh: node_in_graph h G = true).
+           { unfold get_indegree_zero in Hd. destruct G as [V E].
+              assert (H: In h (filter (fun v : node => get_indegree v (V, E) =? 0) V)).
+              { rewrite Hd. simpl. left. reflexivity. }
+              apply filter_true in H. destruct H as [H _]. simpl.
+              apply member_In_equiv. apply H. }
+           destruct Hmem as [Hhu | Hind].
+           ++ unfold get_indegree_zero in Hd. rewrite Hhu in Hmemh. apply Hmemh.
+           ++ specialize IH with (sorted := r) (G := (remove_node_from_graph G h)).
+              apply IH in Hind. destruct G as [V E].
+              ** simpl in Hind. unfold remove_node in Hind.
+                 apply member_In_equiv in Hind. apply filter_true in Hind. destruct Hind as [Hind _].
+                 simpl. apply member_In_equiv. apply Hind.
+              ** destruct G as [V E]. simpl in Hiters. simpl.
+                 assert (H: S (length (remove_node h V)) <= length V).
+                 { unfold remove_node. apply filter_length_membership. simpl in Hmemh. apply member_In_equiv. apply Hmemh. }
+                 lia.
+              ** apply Hr.
+        -- discriminate Hts.
+  - intros Hnode. generalize dependent G. generalize dependent sorted.
+    induction iters as [| iters' IH].
+    + intros sorted G Hiters Hts Hnode.
+      destruct G as [V E]. simpl in Hiters. simpl in Hnode.
+      destruct (length V) as [| l] eqn:Hl.
+      * destruct V as [| h t] eqn:HV.
+        -- simpl in Hnode. discriminate Hnode.
+        -- simpl in Hl. discriminate Hl.
+      * lia.
+    + intros sorted G Hiters Hts Hnode. simpl in Hts.
+      destruct (get_indegree_zero G) as [| h t] eqn:Hd.
+      * discriminate Hts.
+      * destruct (topological_sort_helper (remove_node_from_graph G h) iters') as [r|] eqn:Hr.
+        -- inversion Hts. destruct G as [V E]. simpl in Hnode.
+           destruct (u =? h) as [|] eqn:Huh.
+           ++ apply eqb_eq in Huh. rewrite Huh. simpl. left. reflexivity.
+           ++ assert (Hmem: node_in_graph u (remove_node_from_graph (V, E) h) = true).
+              { simpl. unfold remove_node. apply member_In_equiv.
+                apply filter_true. split.
+                - apply member_In_equiv. apply Hnode.
+                - rewrite Huh. simpl. reflexivity. }
+              specialize IH with (sorted := r) (G := (remove_node_from_graph (V, E) h)).
+              simpl. right. apply IH.
+              ** simpl in Hiters. simpl.
+                 assert (Hmemh: node_in_graph h (V, E) = true).
+                 { unfold get_indegree_zero in Hd.
+                    assert (H: In h (filter (fun v : node => get_indegree v (V, E) =? 0) V)).
+                    { rewrite Hd. simpl. left. reflexivity. }
+                    apply filter_true in H. destruct H as [H _]. simpl.
+                    apply member_In_equiv. apply H. }
+                 assert (H: S (length (remove_node h V)) <= length V).
+                 { unfold remove_node. apply filter_length_membership. simpl in Hmemh. apply member_In_equiv. apply Hmemh. }
+                 lia.
+              ** apply Hr.
+              ** apply Hmem.
+        -- discriminate Hts.
+Qed.
+
+Lemma topo_sort_contains_nodes: forall (G: graph) (sorted: nodes),
+  topological_sort G = Some sorted ->
+  forall (u: node), (In u sorted <-> node_in_graph u G = true).
+Proof.
+  intros G sorted Hts.
+  intros u.
+  apply topo_sort_contains_nodes_helper with (iters := (num_nodes G)).
+  split.
+  - apply le_n.
+  - destruct G as [V E]. unfold topological_sort in Hts. simpl. apply Hts.
+Qed.
+
+Lemma topo_sort_contains_nodes_exactly_once: forall (G: graph) (sorted: nodes),
+  G_well_formed G = true /\ topological_sort G = Some sorted -> 
+  forall (u: node), node_in_graph u G = true -> count u sorted = 1.
+Proof.
+  intros G ts [Hwf Hts].
+  assert (HV: forall (u: node), In u (nodes_in_graph G) -> count u (nodes_in_graph G) = 1).
+  { intros u Hmem. destruct G as [V E].
+    unfold G_well_formed in Hwf. apply split_and_true in Hwf. destruct Hwf as [Hwf _]. apply split_and_true in Hwf. destruct Hwf as [_ Hwf].
+    apply forallb_true_iff_mem with (x := u) in Hwf.
+    - simpl. apply eqb_eq in Hwf. apply Hwf.
+    - simpl in Hmem. apply Hmem. }
+  assert (HVts: forall (u: node), count u (nodes_in_graph G) = count u ts).
+  { intros u.
+    apply topo_sort_length_correct in Hts as Hlen.
+    generalize dependent G. induction ts as [| h t IH].
+    - intros G Hwf Hts Hu Hlen. simpl. simpl in Hlen. destruct G as [V E]. destruct V as [| h1 t1].
+      + simpl. reflexivity.
+      + discriminate Hlen.
+    - intros G Hwf Hts Hnode Hlen. simpl.
+      specialize IH with (G := remove_node_from_graph G h).
+      assert (H: count u (nodes_in_graph (remove_node_from_graph G h)) = count u t).
+      { apply IH.
+        - apply remove_node_preserves_well_formed. apply Hwf.
+        - apply topo_sort_subgraph.
+          + split. apply Hwf.
+            apply topo_sort_contains_nodes with (u := h) in Hts. apply Hts. simpl. left. reflexivity.
+          + apply Hts.
+        - intros u1 Hmem. destruct G as [V E]. simpl in Hmem. simpl.
+          unfold remove_node in Hmem. apply filter_true in Hmem. destruct Hmem as [Hmem Huu1].
+          simpl in Hnode. specialize Hnode with (u := u1). apply Hnode in Hmem.
+          unfold remove_node. 
+          assert (H1: count u1 V = count u1 (filter (fun v : nat => negb (v =? h)) V)).
+          { apply count_filter. apply Huu1. }
+          rewrite <- H1. apply Hmem.
+        - destruct G as [V E]. simpl. simpl in Hnode.
+          specialize Hnode with (u := h). simpl in Hlen.
+          assert (H1: length V = S (length (filter (fun v : nat => negb (v =? h)) V))).
+          { apply count_length. apply Hnode.
+            apply topo_sort_contains_nodes with (u := h) in Hts. simpl in Hts.
+            apply member_In_equiv. apply Hts. left. reflexivity. }
+          rewrite H1 in Hlen. inversion Hlen. unfold remove_node. apply H0. }
+      destruct (h =? u) as [|] eqn:Hhu.
+      + destruct G as [V E]. simpl. simpl in H. simpl in Hnode.
+        assert (HcV: count u V = 1).
+        { apply topo_sort_contains_nodes with (u := h) in Hts. simpl in Hts.
+          specialize Hnode with (u := u). apply Hnode.
+          apply member_In_equiv. apply eqb_eq in Hhu. rewrite <- Hhu. apply Hts. left. reflexivity. }
+        assert (Hct: count u t = 0).
+        { rewrite <- H. unfold remove_node. apply eqb_eq in Hhu. rewrite Hhu. apply count_remove_element. }
+        rewrite HcV. rewrite Hct. reflexivity.
+      + destruct G as [V E]. simpl. simpl in H. unfold remove_node in H.
+        rewrite <- H. apply count_filter. rewrite eqb_sym. rewrite Hhu. simpl. reflexivity. }
+  intros u H.
+  specialize HVts with (u := u). rewrite <- HVts.
+  specialize HV with (u := u). apply HV. destruct G as [V E].
+  simpl in H. simpl. apply member_In_equiv. apply H.
+Qed.
+
+Theorem topo_sort_correct: forall (G: graph) (u v: node) (sorted: nodes),
+  G_well_formed G = true /\ topological_sort G = Some sorted /\ edge_in_graph (u, v) G = true
+  -> exists (i j: nat), Some i = index sorted u /\ Some j = index sorted v /\ i < j.
+Proof.
+Admitted.
+
+Corollary topo_sort_parents: forall (G: graph) (c p: node) (sorted: nodes),
+  G_well_formed G = true /\ topological_sort G = Some sorted
+  -> In p (find_parents c G)
+  -> exists (i j: nat), Some i = index sorted p /\ Some j = index sorted c /\ i < j.
+Proof. 
+  intros G c p sorted. intros [Hwf Hts].
+  intros Hmem. apply edge_from_parent_to_child in Hmem.
+  apply topo_sort_correct with (G := G) (u := p) (v := c) (sorted := sorted).
+  repeat split.
+  - apply Hwf.
+  - apply Hts.
+  - apply Hmem.
+Qed.
+
+Lemma topo_sort_first_node_no_parents: forall (G: graph) (u: node) (ts: nodes),
+  G_well_formed G = true /\ topological_sort G = Some (u :: ts) -> find_parents u G = [].
+Proof.
+  intros G u ts [Hwf Hts].
+  destruct (find_parents u G) as [| h t] eqn:HP.
+  - reflexivity.
+  - (* contradiction: u is first in topological sort *)
+    assert (Hcontra: exists (i j: nat), Some i = index (u :: ts) h /\ Some j = index (u :: ts) u /\ i < j).
+    { apply topo_sort_parents with (G := G).
+      - split. apply Hwf. apply Hts.
+      - rewrite HP. simpl. left. reflexivity. }
+    destruct Hcontra as [i [j [Hi [Hj Hij]]]].
+    simpl in Hj. rewrite eqb_refl in Hj. inversion Hj. rewrite H0 in Hij. lia.
+Qed.
+
+Lemma topo_sort_parents_before: forall (G: graph) (h: node) (tsp t: nodes),
+  G_well_formed G = true /\ topological_sort G = Some (tsp ++ h :: t)
+  -> forall (v: node), In v (find_parents h G) -> In v tsp.
+Proof.
+  intros G h tsp t [Hwf Hts] p Hp.
+  apply topo_sort_parents with (sorted := (tsp ++ h :: t)) in Hp.
+  - (* i < j, so p must appear in tsp *)
+    destruct Hp as [i [j [Hi [Hj Hij]]]].
+    assert (Hmem: ~(In h tsp)).
+    { intros Hhtsp.
+      (* contradict that h appears only once in the topological sort of G *)
+      assert (Hc: count h (tsp ++ h :: t) >= 2).
+      { apply member_count_at_least_1 in Hhtsp.
+        rewrite count_app. simpl. rewrite eqb_refl. lia. }
+      assert (Hc2: count h (tsp ++ h :: t) = 1).
+      { apply topo_sort_contains_nodes_exactly_once with (G := G).
+        - split. apply Hwf. apply Hts.
+        - apply topo_sort_contains_nodes with (u := h) in Hts. apply Hts.
+          apply membership_append_r. simpl. left. reflexivity. }
+      lia. }
+    assert (Hj2: index (tsp ++ h :: t) h = Some (length tsp + 0)).
+    { apply index_append with (l1 := tsp) (l2 := h :: t) (i := 0). split.
+      - apply Hmem.
+      - simpl. rewrite eqb_refl. reflexivity. }
+    rewrite Hj2 in Hj. inversion Hj. rewrite add_0_r in H0. rewrite H0 in Hij.
+    assert (Hptsp: index tsp p = Some i).
+    { apply index_append_2 with (l2 := h :: t). split.
+      - symmetry. apply Hi.
+      - apply Hij. }
+    apply index_exists. exists i. symmetry. apply Hptsp.
+  - split.
+    + apply Hwf.
+    + apply Hts.
+Qed.
